src/HaskCoreVars.v
@@ -5,10 +5,13 @@
 Generalizable All Variables.
 Require Import Preamble.
 Require Import General.
+Require Import Coq.Strings.String.
 
 (* GHC uses a single type for expression variables, type variables, and coercion variables; this is that type *)
 Variable CoreVar          : Type.                                               Extract Inlined Constant CoreVar    => "Var.Var".
 Variable coreVar_eq       : forall (a b:CoreVar), sumbool (a=b) (not (a=b)).    Extract Inlined Constant coreVar_eq => "(==)".
+Variable coreVarToString  : CoreVar      -> string.  Extract Inlined Constant coreVarToString         => "outputableToString".
 Axiom    coreVar_eq_refl  : forall v, (coreVar_eq v v) = (left _ (refl_equal v)).
 Instance CoreVarEqDecidable : EqDecidable CoreVar := { eqd_dec            := coreVar_eq }.
-
+Instance CoreVarToString : ToString CoreVar :=
+  { toString := coreVarToString }.
