src/HaskWeakToStrong.v
@@ -17,17 +17,23 @@ Require Import HaskWeak.
 Require Import HaskStrongTypes.
 Require Import HaskStrong.
 Require Import HaskCoreTypes.
+Require Import HaskCoreVars.
 
-Definition upφ {Γ}(tv:WeakTypeVar)(φ:WeakTypeVar -> HaskTyVar Γ) : (WeakTypeVar -> HaskTyVar ((tv:Kind)::Γ)) :=
-  fun tv' =>
+Open Scope string_scope.
+Definition TyVarResolver Γ   := forall wt:WeakTypeVar, HaskTyVar Γ wt.
+Definition CoVarResolver Γ Δ := forall wt:WeakCoerVar, HaskCoVar Γ Δ.
+
+Definition upφ {Γ}(tv:WeakTypeVar)(φ:TyVarResolver Γ) : TyVarResolver ((tv:Kind)::Γ).
+  unfold TyVarResolver.
+  refine (fun tv' =>
     if eqd_dec tv tv' 
-    then FreshHaskTyVar (tv:Kind)
-    else fun TV ite => φ tv' TV (weakITE ite).
+    then let fresh := @FreshHaskTyVar Γ tv in _
+    else fun TV ite => φ tv' TV (weakITE ite)).
+  rewrite <- _H; apply fresh.
+  Defined.
 
-
-
-Definition upφ' {Γ}(tvs:list WeakTypeVar)(φ:WeakTypeVar -> HaskTyVar Γ)
-  : (WeakTypeVar -> HaskTyVar (app (map (fun tv:WeakTypeVar => tv:Kind) tvs) Γ)).
+Definition upφ' {Γ}(tvs:list WeakTypeVar)(φ:TyVarResolver Γ)
+  : (TyVarResolver (app (map (fun tv:WeakTypeVar => tv:Kind) tvs) Γ)).
   induction tvs.
   apply φ.    
   simpl.
@@ -35,56 +41,35 @@ Definition upφ' {Γ}(tvs:list WeakTypeVar)(φ:WeakTypeVar -> HaskTyVar Γ)
   apply IHtvs.
   Defined.
 
-Open Scope string_scope.
-
-Fixpoint weakTypeToType {Γ:TypeEnv}(φ:WeakTypeVar -> HaskTyVar Γ)(t:WeakType) : HaskType Γ :=
-    match t with
-      | WTyVarTy  v       => fun TV env => @TVar TV (φ v TV env)
-      | WCoFunTy t1 t2 t3 => (weakTypeToType φ t1) ∼∼ (weakTypeToType φ t2) ⇒ (weakTypeToType φ t3)
-      | WFunTyCon         => fun TV env => TArrow
-      | WTyCon      tc    => fun TV env => TCon tc
-      | WTyFunApp   tc lt => fun TV env => fold_left TApp (map (fun t => weakTypeToType φ t TV env) lt) (TCon tc) (* FIXME *)
-      | WClassP   c lt    => fun TV env => fold_left TApp (map (fun t=> weakTypeToType φ t TV env) lt) (TCon (classTyCon c))
-      | WIParam _ ty      => weakTypeToType φ ty
-      | WForAllTy wtv t   => (fun TV env => TAll (wtv:Kind) (fun tv => weakTypeToType (@upφ Γ wtv φ) t TV (tv:::env)))
-      | WAppTy  t1 t2     => fun TV env => TApp (weakTypeToType φ t1 TV env) (weakTypeToType φ t2 TV env)
-      | WCodeTy ec tbody  => fun TV env => TCode (TVar (φ ec TV env)) (weakTypeToType φ tbody TV env)
-    end.
-
-
-Definition substPhi0 {Γ:TypeEnv}(κ:Kind)(θ:HaskType Γ) : HaskType (κ::Γ) -> HaskType Γ.
+Definition substPhi {Γ:TypeEnv}(κ κ':Kind)(θ:HaskType Γ κ) : HaskType (κ::Γ) κ' -> HaskType Γ κ'.
   intro ht.
   refine (substT _ θ).
   clear θ.
   unfold HaskType in ht.
   intros.
   apply ht.
-  apply vec_cons; [ idtac | apply env ].
+  apply ICons; [ idtac | apply env ].
   apply X.
   Defined.
 
-Definition substPhi {Γ:TypeEnv}(κ:list Kind)(θ:vec (HaskType Γ) (length κ)) : HaskType (app κ Γ) -> HaskType Γ.
-  induction κ.
+Definition substφ {Γ:TypeEnv}(lk:list Kind)(θ:IList _ (fun κ => HaskType Γ κ) lk){κ} : HaskType (app lk Γ) κ -> HaskType Γ κ.
+  induction lk.
   intro q; apply q.
   simpl.
   intro q.
-  apply IHκ.
+  apply IHlk.
   inversion θ; subst; auto.
   inversion θ; subst.
-  apply (substPhi0 _ (weakT' X) q).
-  Defined.
-
-Definition substφ {Γ}{n}(ltypes:vec (HaskType Γ) n)(Γ':vec _ n)(ht:HaskType (app (vec2list Γ') Γ)) : HaskType Γ.
-  apply (@substPhi Γ (vec2list Γ')).
-  rewrite vec2list_len.
-  apply ltypes.
-  apply ht.
+  eapply substPhi.
+  eapply weakT'.
+  apply X.
+  apply q.
   Defined.
 
 (* this is a StrongAltCon plus some stuff we know about StrongAltCons which we've built ourselves *)
 Record StrongAltConPlusJunk {tc:TyCon} :=
 { sacpj_sac : @StrongAltCon tc
-; sacpj_φ   : forall Γ          (φ:WeakTypeVar -> HaskTyVar Γ  ),  (WeakTypeVar -> HaskTyVar (sac_Γ sacpj_sac Γ))
+; sacpj_φ   : forall Γ          (φ:TyVarResolver Γ  ),  (TyVarResolver (sac_Γ sacpj_sac Γ))
 ; sacpj_ψ   : forall Γ Δ atypes (ψ:WeakCoerVar -> HaskCoVar Γ Δ),
                 (WeakCoerVar -> HaskCoVar _ (sac_Δ sacpj_sac Γ atypes (weakCK'' Δ)))
 }.
@@ -92,11 +77,11 @@ Implicit Arguments StrongAltConPlusJunk [ ].
 Coercion sacpj_sac : StrongAltConPlusJunk >-> StrongAltCon. 
 
 (* yes, I know, this is really clumsy *)
-Variable emptyφ : WeakTypeVar -> HaskTyVar nil.
+Variable emptyφ : TyVarResolver nil.
   Extract Inlined Constant emptyφ => "(\x -> Prelude.error ""encountered unbound tyvar!"")".
 
 Definition mkPhi (lv:list WeakTypeVar)
-  : (WeakTypeVar -> HaskTyVar (map (fun x:WeakTypeVar => x:Kind) lv)).
+  : (TyVarResolver (map (fun x:WeakTypeVar => x:Kind) lv)).
   set (upφ'(Γ:=nil) lv emptyφ) as φ'.
   rewrite <- app_nil_end in φ'.
   apply φ'.
@@ -105,10 +90,134 @@ Definition mkPhi (lv:list WeakTypeVar)
 Definition dataConExKinds dc := vec_map (fun x:WeakTypeVar => (x:Kind)) (list2vec (dataConExTyVars dc)).
 Definition tyConKinds     tc := vec_map (fun x:WeakTypeVar => (x:Kind)) (list2vec (tyConTyVars tc)).
 
+Definition fixkind {κ}(tv:WeakTypeVar) := weakTypeVar tv κ.
+Notation " ` x " := (@fixkind _ x) (at level 100).
+
+Ltac matchThings T1 T2 S :=
+  destruct (eqd_dec T1 T2) as [matchTypeVars_pf|];
+   [ idtac | apply (Error (S +++ T1 +++ " " +++ T2)) ].
+
+Definition mkTAll' {κ}{Γ} : HaskType (κ :: Γ) ★ -> (forall TV (ite:InstantiatedTypeEnv TV Γ), TV κ -> RawHaskType TV ★).
+  intros.
+  unfold InstantiatedTypeEnv in ite.
+  apply X.
+  apply (X0::::ite).
+  Defined.
+
+Definition mkTAll {κ}{Γ} : HaskType (κ :: Γ) ★ -> HaskType Γ ★.
+  intro.
+  unfold HaskType.
+  intros.
+  apply (TAll κ).
+  eapply mkTAll'.
+  apply X.
+  apply X0.
+  Defined.
+
+Definition weakTypeToType : forall {Γ:TypeEnv}(φ:TyVarResolver Γ)(t:WeakType), ???(HaskTypeOfSomeKind Γ).
+  refine (fix weakTypeToType {Γ:TypeEnv}(φ:TyVarResolver Γ)(t:WeakType) {struct t} : ???(HaskTypeOfSomeKind Γ) :=
+  match t with
+    | WFunTyCon         => let case_WFunTyCon := tt in OK (haskTypeOfSomeKind (fun TV ite => TArrow))
+    | WTyCon      tc    => let case_WTyCon := tt    in _
+    | WClassP   c lt    => let case_WClassP := tt   in Error "weakTypeToType: WClassP not implemented"
+    | WIParam _ ty      => let case_WIParam := tt   in Error "weakTypeToType: WIParam not implemented"
+    | WAppTy  t1 t2     => let case_WAppTy := tt    in weakTypeToType _ φ t1 >>= fun t1' => weakTypeToType _ φ t2 >>= fun t2' => _
+    | WTyVarTy  v       => let case_WTyVarTy := tt  in _
+    | WForAllTy wtv t   => let case_WForAllTy := tt in weakTypeToType _ (upφ wtv φ) t >>= fun t => _
+    | WCodeTy ec tbody  => let case_WCodeTy := tt   in weakTypeToType _ φ tbody >>= fun tbody' => _
+    | WCoFunTy t1 t2 t3 => let case_WCoFunTy := tt  in
+      weakTypeToType _ φ t1 >>= fun t1' =>
+      weakTypeToType _ φ t2 >>= fun t2' =>
+      weakTypeToType _ φ t3 >>= fun t3' => _
+    | WTyFunApp   tc lt =>
+      ((fix weakTypeListToTypeList (lk:list Kind) (lt:list WeakType)
+        { struct lt } : ???(forall TV (ite:InstantiatedTypeEnv TV Γ), @RawHaskTypeList TV lk) :=
+        match lt with
+          | nil    => match lk as LK return ???(forall TV (ite:InstantiatedTypeEnv TV Γ), @RawHaskTypeList TV LK) with
+                        | nil => OK (fun TV _ => TyFunApp_nil)
+                        | _   => Error "WTyFunApp not applied to enough types"
+                      end
+          | tx::lt' => weakTypeToType Γ φ tx >>= fun t' =>
+                        match lk as LK return ???(forall TV (ite:InstantiatedTypeEnv TV Γ), @RawHaskTypeList TV LK) with
+                          | nil    => Error "WTyFunApp applied to too many types"
+                          | k::lk' => weakTypeListToTypeList lk' lt' >>= fun rhtl' =>
+                                        let case_weakTypeListToTypeList := tt in _
+                        end
+        end
+      ) (fst (tyFunKind tc)) lt) >>= fun lt' => let case_WTyFunApp := tt in  _
+  end ); clear weakTypeToType.
+
+  destruct case_WTyVarTy.
+    apply OK.
+    exact (haskTypeOfSomeKind (fun TV env => TVar (φ v TV env))).
+
+  destruct case_WAppTy.
+    destruct t1' as  [k1' t1'].
+    destruct t2' as [k2' t2'].
+    destruct k1';
+      try (matchThings k1'1 k2' "Kind mismatch in WAppTy: ";
+        subst; apply OK; apply (haskTypeOfSomeKind (fun TV env => TApp (t1' TV env) (t2' TV env))));
+      apply (Error "Kind mismatch in WAppTy:: ").
+   
+  destruct case_weakTypeListToTypeList.
+    destruct t' as [ k' t' ].
+    matchThings k k' "Kind mismatch in weakTypeListToTypeList".
+    subst.
+    apply (OK (fun TV ite => TyFunApp_cons _ _ (t' TV ite) (rhtl' TV ite))).
+
+  destruct case_WTyFunApp.
+    apply OK.
+    eapply haskTypeOfSomeKind.
+    unfold HaskType; intros.
+    apply TyFunApp.
+    apply lt'.
+    apply X.
+
+  destruct case_WTyCon.
+    apply OK.
+    eapply haskTypeOfSomeKind.
+    unfold HaskType; intros.
+    apply (TCon tc).
+
+  destruct case_WCodeTy.    
+    destruct tbody'.
+    matchThings κ ★ "Kind mismatch in WCodeTy: ".
+    apply OK.
+    eapply haskTypeOfSomeKind.
+    unfold HaskType; intros.
+    apply TCode.
+    apply (TVar (φ (@fixkind ★ ec) TV X)).
+    subst.
+    apply h.
+    apply X.
+
+  destruct case_WCoFunTy.
+    destruct t1' as [ k1' t1' ].
+    destruct t2' as [ k2' t2' ].
+    destruct t3' as [ k3' t3' ].
+    matchThings k1' k2' "Kind mismatch in arguments of WCoFunTy".
+    subst.
+    matchThings k3' ★ "Kind mismatch in result of WCoFunTy".
+    subst.
+    apply OK.
+    apply (haskTypeOfSomeKind (t1' ∼∼ t2' ⇒ t3')).
+
+  destruct case_WForAllTy.
+    destruct t1.
+    matchThings ★  κ "Kind mismatch in WForAllTy: ".
+    subst.
+    apply OK.
+    apply (@haskTypeOfSomeKind _ ★).
+    apply (@mkTAll wtv).
+    apply h.
+    Defined.
+    
+
+
 (* information about a datacon/literal/default which is common to all instances of a branch with that tag *)
 Section StrongAltCon.
   Context (tc : TyCon)(dc:DataCon tc).
-
+(*
 Definition weakTypeToType' {Γ} : vec (HaskType Γ) tc -> WeakType → HaskType (app (vec2list (dataConExKinds dc)) Γ).
   intro avars.
   intro ct.
@@ -186,15 +295,16 @@ Definition mkStrongAltConPlusJunk : StrongAltConPlusJunk tc.
     apply vec_chop' in cenv.
     apply cenv.
     Defined.
+*)
 End StrongAltCon.
-
+(*
 Definition mkStrongAltConPlusJunk' (tc : TyCon)(alt:AltCon) : ???(@StrongAltConPlusJunk tc).
   destruct alt.
   set (c:DataCon _) as dc.
   set ((dataConTyCon c):TyCon) as tc' in *.
   set (eqd_dec tc tc') as eqpf; destruct eqpf;
     [ idtac
-      | apply (Error ("in a case of tycon "+++tyConToString tc+++", found a branch with datacon "+++dataConToString dc)) ]; subst.
+      | apply (Error ("in a case of tycon "+++tc+++", found a branch with datacon "+++dc)) ]; subst.
   apply OK.
   eapply mkStrongAltConPlusJunk.
   simpl in *.
@@ -212,127 +322,20 @@ Definition mkStrongAltConPlusJunk' (tc : TyCon)(alt:AltCon) : ???(@StrongAltConP
             intro; intro φ; apply φ.
             intro; intro; intro; intro ψ; apply ψ.
 Defined.
-
-Fixpoint mLetRecTypesVars {Γ} (mlr:Tree ??(WeakExprVar * WeakExpr)) φ : Tree ??(WeakExprVar * HaskType Γ) :=
+Fixpoint mLetRecTypesVars {Γ} (mlr:Tree ??(WeakExprVar * WeakExpr)) φ : Tree ??(WeakExprVar * HaskType Γ ★) :=
   match mlr with
-  | T_Leaf None         => []
+  | T_Leaf None                         => []
   | T_Leaf (Some ((weakExprVar v t),e)) => [((weakExprVar v t),weakTypeToType φ t)]
-  | T_Branch b1 b2 => ((mLetRecTypesVars b1 φ),,(mLetRecTypesVars b2 φ))
+  | T_Branch b1 b2                      => ((mLetRecTypesVars b1 φ),,(mLetRecTypesVars b2 φ))
   end.
+*)
 
-Open Scope string_scope.
-Definition unlev {Γ:TypeEnv}(lht:LeveledHaskType Γ) : HaskType Γ   := match lht with t @@ l => t end.
-
-Definition Indexed_Bind T f t (e:@Indexed T f t) : forall Q, (forall t, f t -> ???Q) -> ???Q.
-intros.
-destruct e; subst.
-apply (Error error_message).
-apply (X t f0).
-Defined.
-Notation "a >>>= b" := (@Indexed_Bind _ _ _ a _ b) (at level 20).
-
-Definition DoublyIndexed_Bind T f t (e:@Indexed T (fun z => ???(f z)) t) : forall Q, (forall t, f t -> ???Q) -> ???Q.
-  intros.
-  eapply Indexed_Bind.
-  apply e.
-  intros.
-  destruct X0.
-  apply (Error error_message).
-  apply (X t0 f0).
-  Defined.
-
-Notation "a >>>>= b" := (@DoublyIndexed_Bind _ _ _ a _ b) (at level 20).
-
-Ltac matchTypes T1 T2 S :=
-  destruct (eqd_dec T1 T2) as [matchTypes_pf|];
-   [ idtac | apply (Error ("type mismatch in "+++S+++": " +++ (weakTypeToString T1) +++ " and " +++ (weakTypeToString T2))) ].
-Ltac matchTypeVars T1 T2 S :=
-  destruct (eqd_dec T1 T2) as [matchTypeVars_pf|];
-   [ idtac | apply (Error ("type variable mismatch in"+++S)) ].
-Ltac matchLevs L1 L2 S :=
-  destruct (eqd_dec L1 L2) as [matchLevs_pf|];
-   [ idtac | apply (Error ("level mismatch in "+++S)) ].
-
-
-Definition cure {Γ}(ξ:WeakExprVar -> WeakType * list WeakTypeVar)(φ:WeakTypeVar->HaskTyVar Γ)
-  : WeakExprVar->LeveledHaskType Γ :=
-  fun wtv => weakTypeToType φ (fst (ξ wtv)) @@ map φ (snd (ξ wtv)).
 
 Definition weakExprVarToWeakType : WeakExprVar -> WeakType :=
   fun wev => match wev with weakExprVar _ t => t end.
   Coercion weakExprVarToWeakType : WeakExprVar >-> WeakType.
 
-Fixpoint upξ (ξ:WeakExprVar -> WeakType * list WeakTypeVar)
- (evs:list WeakExprVar)
- (lev:list WeakTypeVar) :
-  (WeakExprVar -> WeakType * list WeakTypeVar) :=
-  fun wev =>
-  match evs with
-    | nil  => ξ wev
-    | a::b => if eqd_dec wev a then ((wev:WeakType),lev) else upξ ξ b lev wev
-  end.
-
-Variable weakCoercionToHaskCoercion : forall Γ Δ, WeakCoercion -> HaskCoercion Γ Δ.
-
-Notation "'checkit' ( Y ) X" := (match weakTypeOfWeakExpr Y as CTE return
-                                   CTE=weakTypeOfWeakExpr Y -> forall Γ Δ φ ψ ξ lev, Indexed _ CTE with
-                                | Error s   =>   fun  _ _ _ _ _ _  _   => Indexed_Error _ s
-                                | OK    cte =>  fun cte_pf => (fun x Γ Δ φ ψ ξ lev => Indexed_OK _ _ (x Γ Δ φ ψ ξ lev)) X
-                              end (refl_equal _)) (at level 10).
-
-
-(* equality lemmas I have yet to prove *)
-
-Lemma upξ_lemma Γ ξ v lev φ
-  : cure(Γ:=Γ) (upξ ξ (v :: nil) lev) φ = update_ξ (cure ξ φ) ((v,weakTypeToType φ v @@  map φ lev)::nil).
-  admit.
-  Qed.
-
-(* this is tricky because of the test for ModalBoxTyCon is a type index for tc and because the fold is a left-fold *)
-
-Lemma letrec_lemma : forall Γ ξ φ rb lev,
-let ξ' := upξ ξ (map (@fst _ _) (leaves (mLetRecTypesVars rb φ))) lev in
-(cure ξ' φ) = (
-        update_ξ (cure ξ φ)
-          (map
-             (fun x : WeakExprVar * HaskType Γ =>
-              ⟨fst x, snd x @@  map φ lev ⟩) (leaves (mLetRecTypesVars rb φ)))).
-admit.
-Qed.
-
-Lemma case_lemma1 tc Γ avars' (sac:StrongAltConPlusJunk tc) vars ξ φ lev :
-(@scbwv_ξ WeakExprVar WeakExprVarEqDecidable tc Γ avars'
-        {| scbwv_sac := sac; scbwv_exprvars := vars |} 
-        (@cure Γ ξ φ) (@map WeakTypeVar (HaskTyVar Γ) φ lev))
-      = (cure ξ (sacpj_φ sac Γ φ)).
-  admit.
-  Qed.
-Lemma case_lemma2 tc Γ  (sac:@StrongAltConPlusJunk tc)  φ lev :
-  (map (sacpj_φ sac Γ φ) lev) = weakL' (map φ lev).
-  admit.
-  Qed.
-Lemma case_lemma3 Γ φ t tc   (sac:@StrongAltConPlusJunk tc) :
- (weakT' (weakTypeToType φ t) = weakTypeToType (sacpj_φ sac Γ φ) t).
-        admit.
-  Qed.
-Lemma case_lemma4 Γ φ (tc:TyCon) avars0 : forall Q1 Q2, (@weakTypeToType Γ φ Q2)=Q1 ->
-   fold_left HaskAppT (map (weakTypeToType φ) avars0) Q1 =
-   weakTypeToType φ (fold_left WAppTy avars0 Q2).
-   induction avars0; intros.
-   simpl.
-   symmetry; auto.
-   simpl.
-   set (IHavars0 (HaskAppT Q1 (weakTypeToType φ a)) (WAppTy Q2 a)) as z.
-   rewrite z.
-   reflexivity.
-   rewrite <- H.
-   simpl.
-   auto.
-   Qed.
-
-(* for now... *)
-Axiom assume_all_coercions_well_formed : forall Γ (Δ:CoercionEnv Γ) t1 t2 co, Δ ⊢ᴄᴏ  co : t1 ∼ t2.
-Axiom assume_all_types_well_formed     : forall Γ t x,    Γ ⊢ᴛy t : x.
+(*Variable weakCoercionToHaskCoercion : forall Γ Δ κ, WeakCoercion -> HaskCoercion Γ Δ κ.*)
 
 Definition weakψ {Γ}{Δ:CoercionEnv Γ} {κ}(ψ:WeakCoerVar -> HaskCoVar Γ Δ) :
   WeakCoerVar -> HaskCoVar Γ (κ::Δ).
@@ -343,353 +346,111 @@ Definition weakψ {Γ}{Δ:CoercionEnv Γ} {κ}(ψ:WeakCoerVar -> HaskCoVar Γ Δ
   inversion cenv; auto.
   Defined.
 
-Lemma substRaw {Γ}{κ} : HaskType (κ::Γ) -> (∀ TV, @InstantiatedTypeEnv TV Γ -> TV -> @RawHaskType TV).
-  intro ht.
-  intro TV.
-  intro env.
-  intro tv.
-  apply ht.
-  apply (tv:::env).
+(* attempt to "cast" an expression by simply checking if it already had the desired type, and failing otherwise *)
+Definition castExpr (err_msg:string) {Γ} {Δ} {ξ} {τ} τ' (e:@Expr _ WeakExprVarEqDecidable Γ Δ ξ τ)
+  : ???(@Expr _ WeakExprVarEqDecidable Γ Δ ξ τ').
+  intros.
+  destruct τ  as [τ  l].
+  destruct τ' as [τ' l'].
+  destruct (eqd_dec l l'); [ idtac | apply (Error ("level mismatch in castExpr: "+++err_msg)) ].
+  destruct (eqd_dec τ τ'); [ idtac | apply (Error ("type mismatch in castExpr: " +++err_msg+++" "+++τ+++" and "+++τ')) ].
+  subst.
+  apply OK.
+  apply e.
   Defined.
 
-Lemma substRaw_lemma : forall (Γ:TypeEnv) (φ:WeakTypeVar->HaskTyVar Γ) wt tsubst wtv,
-  substT (substRaw (weakTypeToType (upφ wtv φ) wt)) (weakTypeToType φ tsubst) =
-  weakTypeToType φ (replaceWeakTypeVar wt wtv tsubst).
-  admit.
-  Qed.
+Definition weakTypeToType' : forall {Γ:TypeEnv}(φ:TyVarResolver Γ)(t:WeakType) κ, ???(HaskType Γ κ).
+  intros.
+  set (weakTypeToType φ t) as wt.
+  destruct wt; try apply (Error error_message).
+  destruct h.
+  matchThings κ κ0 "Kind mismatch in weakTypeToType': ".
+  subst.
+  apply OK.
+  apply h.
+  Defined.
 
 Definition weakExprToStrongExpr : forall
-    (ce:WeakExpr)
     (Γ:TypeEnv)
     (Δ:CoercionEnv Γ)
-    (φ:WeakTypeVar->HaskTyVar Γ)
-    (ψ:WeakCoerVar->HaskCoVar Γ Δ)
-    (ξ:WeakExprVar->WeakType * list WeakTypeVar)
-    (lev:list WeakTypeVar)
-    ,
-    Indexed (fun t' => ???(@Expr _ WeakExprVarEqDecidable Γ Δ (cure ξ φ) (weakTypeToType φ t' @@ (map φ lev))))
-       (weakTypeOfWeakExpr ce).
+    (φ:TyVarResolver Γ)
+    (ψ:CoVarResolver Γ Δ)
+    (ξ:WeakExprVar -> LeveledHaskType Γ ★)
+    (τ:HaskType Γ ★)
+    (lev:HaskLevel Γ),
+    WeakExpr -> ???(Expr Γ Δ ξ (τ @@ lev) ).
   refine ((
-    fix weakExprToStrongExpr (ce:WeakExpr) {struct ce} : forall Γ Δ φ ψ ξ lev,
-      Indexed (fun t' => ???(Expr Γ Δ (cure ξ φ) (weakTypeToType φ t' @@ (map φ lev)))) (weakTypeOfWeakExpr ce) :=
-    (match ce as CE return (forall Γ Δ φ ψ ξ lev, Indexed _ (weakTypeOfWeakExpr CE))
-      with
-    | WEVar   v                   => let case_WEVar := tt in checkit (WEVar   v) (fun Γ Δ φ ψ ξ lev => _)
-    | WELit   lit                 => let case_WELit := tt in checkit (WELit   lit) (fun Γ Δ φ ψ ξ lev => _)
-    | WEApp   e1 e2               => let case_WEApp := tt in checkit (WEApp   e1 e2)       (fun Γ Δ φ ψ ξ lev =>
-        weakExprToStrongExpr e1 Γ Δ φ ψ ξ lev >>>>= fun te1 e1' => 
-          ((weakExprToStrongExpr e2 Γ Δ φ ψ ξ lev) >>>>= fun te2 e2' => _))
-    | WETyApp e t                 => let case_WETyApp := tt in
-      checkit (WETyApp e t) (fun Γ Δ φ ψ ξ lev => weakExprToStrongExpr e Γ Δ φ ψ ξ lev >>>>= fun te' e' => _)
-    | WECoApp e t                 => let case_WECoApp := tt in
-      checkit (WECoApp e t) (fun Γ Δ φ ψ ξ lev => weakExprToStrongExpr e Γ Δ φ ψ ξ lev >>>>= fun te' e' => _)
-    | WELam   ev e                => let case_WELam   := tt in 
-      checkit (WELam   ev e) (fun Γ Δ φ ψ ξ lev =>
-        let ξ' := @upξ ξ (ev::nil) lev in
-        weakExprToStrongExpr e Γ Δ φ ψ ξ' lev >>>>= fun te' e' => _)
-    | WECoLam cv e                => let case_WECoLam := tt in
-      checkit (WECoLam cv e) (fun Γ Δ φ ψ ξ lev => (fun e' => _) (weakExprToStrongExpr e))
-    | WEBrak  ec e tbody              => let case_WEBrak  := tt in
-      checkit (WEBrak  ec e tbody) (fun Γ Δ φ ψ ξ lev => weakExprToStrongExpr e Γ Δ φ ψ ξ (ec::lev) >>>>= fun te' e' => _)
-    | WEEsc   ec e tbody              => 
-      checkit (WEEsc   ec e tbody) (fun Γ Δ φ ψ ξ lev =>
-        match lev as LEV return lev=LEV -> _ with
-          | nil       => let case_WEEsc_bogus   := tt in _
-          | ec'::lev' => fun ecpf =>  weakExprToStrongExpr e Γ Δ φ ψ ξ lev' >>>>= fun te' e' => let case_WEEsc   := tt in _
-        end (refl_equal _))
-    | WETyLam tv e                => let case_WETyLam := tt in
-      checkit (WETyLam tv e) (fun Γ Δ φ ψ ξ lev => (fun e' => _) (weakExprToStrongExpr e))
-    | WENote  n e                 => let case_WENote := tt in
-      checkit (WENote  n e) (fun Γ Δ φ ψ ξ lev => weakExprToStrongExpr e Γ Δ φ ψ ξ lev >>>>= fun te' e' => _)
-    | WECast  e co                => let case_WECast := tt in
-      checkit (WECast  e co) (fun Γ Δ φ ψ ξ lev => weakExprToStrongExpr e Γ Δ φ ψ ξ lev >>>>= fun te' e' => _)
-    | WELet   v ve  e             => let case_WELet   := tt in 
-      checkit (WELet   v ve e) (fun Γ Δ φ ψ ξ lev =>
-        let ξ' := upξ ξ (v::nil) lev in
-          ((weakExprToStrongExpr e Γ Δ φ ψ ξ lev)
-            >>>>= (fun te' e' => ((weakExprToStrongExpr ve Γ Δ φ ψ ξ' lev) >>>>= (fun vet' ve' => _)))))
+    fix weakExprToStrongExpr 
+    (Γ:TypeEnv)
+    (Δ:CoercionEnv Γ)
+    (φ:TyVarResolver Γ)
+    (ψ:CoVarResolver Γ Δ)
+    (ξ:WeakExprVar -> LeveledHaskType Γ ★)
+    (τ:HaskType Γ ★)
+    (lev:HaskLevel Γ)
+    (we:WeakExpr) : ???(@Expr _ WeakExprVarEqDecidable Γ Δ ξ (τ @@ lev) )  :=
+    match we with
 
-    | WELetRec rb   e             => 
-      checkit (WELetRec rb e) (fun Γ Δ φ ψ ξ lev =>
-let ξ' := upξ ξ (map (@fst _ _) (leaves (mLetRecTypesVars rb φ))) lev in
-          ((fix mLetRecBindingsToELetRecBindings (mlr:Tree ??(WeakExprVar * WeakExpr)) : forall Γ Δ φ ψ ξ lev,
-            ???(ELetRecBindings Γ Δ (cure ξ φ) (map φ lev) (mLetRecTypesVars mlr φ)) :=
-            match mlr as MLR return forall Γ Δ φ ψ ξ lev,
-              ???(ELetRecBindings Γ Δ (cure ξ φ) (map φ lev) (mLetRecTypesVars MLR φ)) with
-              | T_Leaf None       => fun Γ Δ φ ψ ξ lev => OK (ELR_nil _ _ _ _)
-              | T_Leaf (Some  (cv,e)) => fun Γ Δ φ ψ ξ lev =>
-                let case_mlr_leaf := tt in weakExprToStrongExpr e Γ Δ φ ψ ξ lev >>>>= fun me => _
-              | T_Branch b1 b2   =>
-                fun Γ Δ φ ψ ξ lev  => 
-                  mLetRecBindingsToELetRecBindings b1 Γ Δ φ ψ ξ lev >>= fun x1' =>
-                    mLetRecBindingsToELetRecBindings b2 Γ Δ φ ψ ξ lev >>= fun x2' =>
-                      OK (ELR_branch _ _ _ _ _ _ x1' x2')
-            end) rb Γ Δ φ ψ ξ' lev) >>= fun rb' => (weakExprToStrongExpr e Γ Δ φ ψ ξ' lev)
-          >>>>= fun et' e' =>
-      let case_MLLetRec := tt in _)
-      
-    | WECase  e tbranches tc avars alts =>
-      checkit (WECase  e tbranches  tc avars alts) (fun Γ Δ φ ψ ξ lev =>
-        list2vecOrFail avars _ (fun _ _ => "number of types provided did not match the tycon's number of universal tyvars in Case")
-        >>= fun avars0 => 
-          let avars' := vec_map (@weakTypeToType Γ φ) avars0 in
-          let tbranches' := @weakTypeToType Γ φ tbranches in
-            ((fix caseBranches (alts:Tree ??(AltCon*list WeakTypeVar*list WeakCoerVar*list WeakExprVar*WeakExpr))
-              :
-               ???(Tree ??{ scb : StrongCaseBranchWithVVs WeakExprVar _ tc avars'
-                            & Expr (sac_Γ scb Γ)
-                                   (sac_Δ scb Γ avars' (weakCK'' Δ))
-                                   (scbwv_ξ scb (cure ξ φ) (map φ lev))
-                                   (weakLT' (tbranches'@@(map φ lev))) }) :=
-              match alts with
-              | T_Leaf None             => OK []
-              | T_Branch b1 b2          => caseBranches b1 >>= fun b1' => caseBranches b2 >>= fun b2' => OK (b1',,b2')
-              | T_Leaf (Some (alt,tvars,cvars,vvars,e')) =>
-                mkStrongAltConPlusJunk' tc alt >>= fun sac =>
-                list2vecOrFail vvars (sac_numExprVars (sac:@StrongAltCon tc))
-                (fun _ _ => "number of expression variables provided did not match the datacon's number of fields") >>= fun vars =>
-                  let scb := @Build_StrongCaseBranchWithVVs WeakExprVar _ tc Γ avars' sac vars in
-                  let rec 
-                    := @weakExprToStrongExpr e'
-                    (sac_Γ scb Γ)
-                    (sac_Δ scb Γ avars' (weakCK'' Δ))
-                    (sacpj_φ sac Γ φ)
-                    (let case_psi := tt in _)
-                    ξ
-                    lev in (let case_ECase_leaf := tt in _)
-              end
-              ) alts) >>= fun alts' =>
-            weakExprToStrongExpr e Γ Δ φ ψ ξ lev >>>>= fun te' e' =>
-              let case_ECase := tt in _)
-     end))); clear weakExprToStrongExpr.
+    | WEVar   v                         => castExpr "WEVar" (τ @@ lev) (EVar Γ Δ ξ v)
 
-    destruct case_WEVar; intros.
-      matchTypes cte (fst (ξ v)) "HaskWeak EVar".
-      rewrite matchTypes_pf.
-      matchLevs (snd (ξ v)) lev "HaskWeak EVar".
-      rewrite <- matchLevs_pf.
-      apply OK.
-      apply (EVar _ _ (cure ξ φ)).
+    | WELit   lit                       => castExpr "WELit" (τ @@ lev) (ELit Γ Δ ξ lit lev)
 
-    destruct case_WELit; intros.
-      matchTypes (WTyCon (haskLiteralToTyCon lit)) cte "HaskWeak ELit".
-      rewrite <- matchTypes_pf.
-      apply OK.
-      replace (weakTypeToType φ (WTyCon (haskLiteralToTyCon lit))) with (@literalType lit Γ); [ idtac | reflexivity].
-      apply ELit.
+    | WELam   ev e                      => weakTypeToType' φ ev ★ >>= fun tv =>
+                                             weakTypeOfWeakExpr e >>= fun t =>
+                                               weakTypeToType' φ t ★ >>= fun τ' =>
+                                                 weakExprToStrongExpr Γ Δ φ ψ (update_ξ ξ ((ev,tv@@lev)::nil)) τ' _ e >>= fun e' =>
+                                                   castExpr "WELam" _ (ELam Γ Δ ξ tv _ _ ev e')
 
-    destruct case_WELet; intros.
-      unfold ξ' in ve'.
-      matchTypes te' v "HaskWeak ELet".
-      rename matchTypes_pf into matchTypes_pf'.
-      matchTypes cte vet' "HaskWeak ELet".
-      apply OK.
-      eapply ELet.
-      apply e'.
-      rewrite matchTypes_pf'.
-      rewrite matchTypes_pf.
-      rewrite upξ_lemma in ve'.
-      apply ve'.
+    | WEBrak  ec e tbody                => weakExprToStrongExpr Γ Δ φ ψ ξ τ ((φ (`ec))::lev) e >>= fun e' =>
+                                             castExpr "WEBrak" _ (EBrak _ _ _ (φ (`ec)) _ lev e')
 
-    destruct case_mlr_leaf; intros.
-      simpl.
-      destruct cv.
-      matchTypes me w "HaskWeak LetRec".
-      apply OK.
-      apply ELR_leaf.
-      rewrite <- matchTypes_pf.
-      apply X.
+    | WEEsc   ec e tbody                => weakTypeToType' φ tbody ★ >>= fun tbody' =>
+                                           match lev with
+                                             | nil       => Error "ill-leveled escapification"
+                                             | ec'::lev' => weakExprToStrongExpr Γ Δ φ ψ ξ (<[ φ (`ec) |- tbody' ]>) lev e
+                                               >>= fun e' =>
+                                                              castExpr "WEEsc" (τ@@lev) (EEsc _ _ _ (φ (`ec)) _ lev e')
+                                           end
+    | WENote  n e                       => weakExprToStrongExpr Γ Δ φ ψ ξ τ lev e >>= fun e' => OK (ENote _ _ _ _ n e')
 
-    destruct case_MLLetRec; intros.
-      matchTypes et' cte "HaskWeak LetRec".
-      apply OK.
-      unfold ξ' in rb'.
-      rewrite (letrec_lemma Γ ξ φ rb lev) in rb'.
-      apply (@ELetRec WeakExprVar _ Γ Δ (cure ξ φ) (map φ lev) (weakTypeToType φ cte) _ rb').
-      rewrite <- (letrec_lemma Γ ξ φ rb lev).
-      rewrite <- matchTypes_pf.
-      apply e'.
+    | WELet   v ve  ebody               => weakTypeToType' φ v ★  >>= fun tv =>
+                                             weakExprToStrongExpr Γ Δ φ ψ ξ tv lev ve >>= fun ve' =>
+                                               weakExprToStrongExpr Γ Δ φ ψ (update_ξ ξ ((v,tv@@lev)::nil)) τ lev ebody
+                                               >>= fun ebody' =>
+                                                 OK (ELet _ _ _ tv _ lev v ve' ebody')
 
-    destruct case_WECast; intros.
-      apply OK.
-      apply (fun pf => @ECast WeakExprVar _ Γ Δ (cure ξ φ) (weakCoercionToHaskCoercion Γ Δ co) _ _ (map φ lev) pf e').
-      apply assume_all_coercions_well_formed.
+    | WEApp   e1 e2                     => weakTypeOfWeakExpr e2 >>= fun t2 =>
+                                             weakTypeToType' φ t2 ★ >>= fun t2' =>
+                                               weakExprToStrongExpr Γ Δ φ ψ ξ t2' lev e2 >>= fun e2' =>
+                                                 weakExprToStrongExpr Γ Δ φ ψ ξ (t2'--->τ) lev e1 >>= fun e1' =>
+                                                   OK (EApp _ _ _ _ _ _ e1' e2')
 
-    destruct case_WENote; intros.
-      matchTypes te' cte "HaskWeak ENote".
-      apply OK.
-      apply ENote.
-      apply n.
-      rewrite <- matchTypes_pf.
-      apply e'.
+    | WETyLam tv e                      => let φ' := upφ tv φ in
+                                             weakTypeOfWeakExpr e >>= fun te =>
+                                               weakTypeToType' φ' te ★ >>= fun τ' =>
+                                                 weakExprToStrongExpr _ (weakCE Δ) φ' (weakCV○ψ) (weakLT○ξ) τ' (weakL lev) e
+                                                 >>= fun e' =>
+                                                   castExpr "WETyLam1" _ e' >>= fun e'' =>
+                                                     castExpr "WETyLam2" _ (ETyLam Γ Δ ξ tv (mkTAll' τ') lev e'')
 
-    destruct case_WEApp; intros.
-      matchTypes te1 (WAppTy (WAppTy WFunTyCon te2) cte) "HaskWeak EApp".
-      inversion cte_pf.
-      destruct (weakTypeOfWeakExpr e1); try apply (Error error_message).
-      simpl in H0.
-      destruct w; try apply (Error error_message); inversion H0.
-      destruct w1; try apply (Error error_message); inversion H0.
-      destruct w1_1; try apply (Error error_message); inversion H0.
-      clear H0 H1 H2.
-      rewrite matchTypes_pf in e1'.
-      simpl in e1'.
-      rewrite <- H3.
-      apply (OK (EApp _ _ _ _ _ _ e1' e2')).
+    | WETyApp e t                       => weakTypeOfWeakExpr e >>= fun te =>
+                                           match te with
+                                             | WForAllTy wtv te' =>
+                                               let φ' := upφ wtv φ in
+                                                 weakTypeToType' φ' te' ★ >>= fun te'' =>
+                                                   weakExprToStrongExpr Γ Δ φ ψ ξ (mkTAll te'') lev e >>= fun e' =>
+                                                     weakTypeToType' φ t wtv >>= fun t' =>
+                                                       castExpr "WETyApp" _ (ETyApp Γ Δ wtv (mkTAll' te'') t' ξ lev e')
+                                             | _                 => Error ("weakTypeToType: WETyApp body with type "+++te)
+                                           end
 
-    destruct case_WETyApp; intros.
-      inversion cte_pf.
-      destruct (weakTypeOfWeakExpr e); simpl in *; inversion H0.
-      clear H1.
-      destruct w; inversion H0.
-      simpl in cte_pf.
-      clear cte_pf.
-      rename w0 into wt.
-      rename t into tsubst.
-      rename w into wtv.
-      set (@ETyApp WeakExprVar _ Γ Δ wtv
-        (substRaw (weakTypeToType (upφ wtv φ) wt))
-        (weakTypeToType φ tsubst)
-        (cure ξ φ)
-        (map φ lev)
-        (assume_all_types_well_formed _ _ _)
-      ) as q.
+    (* I had all of these working before I switched to a Kind-indexed representation for types; it will take a day or two
+     * to get them back working again *)
+    | WECoApp e t                       => Error "weakExprToStrongExpr: WECoApp  not yet implemented"
+    | WECoLam cv e                      => Error "weakExprToStrongExpr: WECoLam  not yet implemented"
+    | WECast  e co                      => Error "weakExprToStrongExpr: WECast   not yet implemented"
+    | WELetRec rb   e                   => Error "weakExprToStrongExpr: WELetRec not yet implemented"
+    | WECase  e tbranches tc avars alts => Error "weakExprToStrongExpr: WECase   not yet implemented"
+    end)).
+    Defined.
 
-      (* really messy –– but it works! *)
-      matchTypes te' (WForAllTy wtv wt) "HaskWeak ETyApp".
-      apply OK.
-      rewrite substRaw_lemma in q.
-      apply q.
-      clear q H1 H0.
-      rewrite matchTypes_pf in e'.
-      simpl in e'.
-      unfold HaskTAll.
-      unfold substRaw.
-      apply e'.
-
-    destruct case_WECoApp; intros.
-      inversion cte_pf.
-      destruct (weakTypeOfWeakExpr e); simpl in *; inversion H0.
-      clear H1.
-      destruct w; inversion H0.
-      subst.
-      destruct t as [ct1 ct2 cc].
-      set (@ECoApp WeakExprVar _ Γ Δ (weakCoercionToHaskCoercion Γ Δ (weakCoercion ct1 ct2 cc))
-              (weakTypeToType φ ct1) (weakTypeToType φ ct2) (weakTypeToType φ te') (cure ξ φ) (map φ lev)) as q.
-      matchTypes w3 te' "HaskWeak ECoApp".
-      rewrite matchTypes_pf.
-      clear matchTypes_pf.
-      matchTypes (WCoFunTy ct1 ct2 te') te' "HaskWeak ECoApp".
-      apply OK.
-      apply q.
-      apply assume_all_coercions_well_formed.
-      clear q H0 cte_pf.
-      rewrite <- matchTypes_pf in e'.
-      simpl in e'.
-      apply e'.
-
-    destruct case_WELam; intros.
-      simpl in cte_pf.
-      destruct ev as [evv evt].
-      destruct (weakTypeOfWeakExpr e); simpl in cte_pf; inversion cte_pf; try apply (Error error_message).
-      matchTypes te' w "HaskWeak ELam".
-      rewrite <- matchTypes_pf.
-      apply OK.
-      simpl.
-      eapply ELam.
-      apply assume_all_types_well_formed.
-      unfold ξ' in e'.
-      rewrite upξ_lemma in e'.
-      apply e'.
-
-    destruct case_WETyLam; intros.
-      inversion cte_pf.
-      destruct tv.
-      destruct (weakTypeOfWeakExpr e).
-      inversion H0.
-      inversion H0.
-      set (e' (k::Γ) (weakCE Δ) (upφ (weakTypeVar c k) φ) (fun x => weakCV (ψ x)) ξ lev) as e''.
-      inversion e''; try apply (Error error_message).
-      inversion X; try apply (Error error_message).
-      apply (Error "FIXME: HaskWeakToStrong: type lambda not yet implemented").
-
-    destruct case_WECoLam; intros.
-      inversion cte_pf.
-      destruct cv.
-      destruct (weakTypeOfWeakExpr e).
-      inversion H0.
-      inversion H0.
-      set (e' Γ (weakTypeToType φ w ∼∼∼ weakTypeToType φ w0 :: Δ) φ (weakψ ψ) ξ lev) as q.
-      inversion q.
-      destruct X; try apply (Error error_message).
-      set (kindOfType (weakTypeToType φ w)) as qq.
-      destruct qq; try apply (Error error_message).
-      apply OK.
-      apply ECoLam with (κ:=k).
-      apply assume_all_types_well_formed.
-      apply assume_all_types_well_formed.
-      fold (@weakTypeToType Γ).
-      apply e0.
-
-    destruct case_WEBrak; intros.
-      simpl in cte_pf.
-      destruct ec as [ecv eck].
-      destruct (weakTypeOfWeakExpr e); inversion cte_pf; try apply (Error error_message).
-      simpl.
-      matchTypes te' w "HaskWeak EBrak".
-      apply OK.
-      apply EBrak.
-      rewrite matchTypes_pf in e'.
-      apply e'.
-
-    destruct case_WEEsc_bogus; intros.
-      apply (Error "attempt to use escape symbol at level zero").
-
-    destruct case_WEEsc; intros.
-      rewrite ecpf.
-      clear ecpf lev.
-      matchTypes te' (WCodeTy ec' cte) "HaskWeak EEsc".
-      apply OK.
-      apply EEsc.
-      rewrite matchTypes_pf in e'.
-      simpl in e'.
-      apply e'.
-
-    destruct case_psi.
-      apply (sacpj_ψ sac Γ Δ avars' ψ).
-
-    destruct case_ECase_leaf.
-      inversion rec; try apply (Error error_message).
-      destruct X; try apply (Error error_message).
-      matchTypes tbranches t "HaskWeak ECase".
-      apply OK.
-      apply T_Leaf.
-      apply Some.
-      apply (existT _ {| scbwv_sac := scb ; scbwv_exprvars := vars |}).
-      simpl.
-      unfold tbranches'.
-      rewrite matchTypes_pf.
-      rewrite case_lemma1.
-      rewrite <- case_lemma2.
-      rewrite case_lemma3.
-      apply e0.
-
-    destruct case_ECase; intros.
-      matchTypes cte tbranches "HaskWeak ECase". 
-      rewrite matchTypes_pf.
-      clear matchTypes_pf.
-      matchTypes te' (fold_left WAppTy (vec2list avars0) (WTyCon tc)) "HaskWeak ECase".
-      apply OK.
-      apply (fun e => @ECase WeakExprVar _ Γ Δ (cure ξ φ) (map φ lev) tc _ _ e alts').
-      unfold caseType.
-      unfold avars'.
-      replace (fold_left HaskAppT (vec2list (vec_map (weakTypeToType φ) avars0)) (HaskTCon tc))
-        with (weakTypeToType φ (fold_left WAppTy (vec2list avars0) (WTyCon tc))).
-      rewrite <- matchTypes_pf.
-      apply e'.
-      symmetry.
-      rewrite <- vec2list_map_list2vec.
-      apply case_lemma4.
-      apply tc.
-      reflexivity.
-      Defined.
